# $Id: ch-rules.n3 1295 2007-05-11 16:52:51Z josd $
#
# see http://www.informatik.uni-ulm.de/pm/fileadmin/pm/home/fruehwirth/drafts/jlp-chr1.ps.gz
#
# PxButton | check with cwm | bash .cwm ch-rules.n3

@prefix log: <http://www.w3.org/2000/10/swap/log#>.
@prefix math: <http://www.w3.org/2000/10/swap/math#>.
@prefix owl: <http://www.w3.org/2002/07/owl#>.
@prefix xsd: <http://www.w3.org/2001/XMLSchema#>.
@prefix rdfs: <http://www.w3.org/2000/01/rdf-schema#>.
@prefix rdf: <http://www.w3.org/1999/02/22-rdf-syntax-ns#>.
@prefix : <http://eulersharp.sourceforge.net/2003/03swap/ch-rules#>.


### Constraint Handling Rules
#
# CHR are essentially a committed-choice language consisting of guarded
# rules that rewrite constraints into simpler ones until they are solved.
# CHR define both simplification of and propagation over user constraints.

:simplification
	a rdf:Property;
	rdfs:domain log:Formula;
	rdfs:range log:Formula;
	rdfs:comment "simplification replaces constraints by simpler constraints while preserving logical equivalence".

:propagation
	a rdf:Property;
	rdfs:domain log:Formula;
	rdfs:range log:Formula;
	rdfs:comment "propagation adds new constraints which are logically redundant but may cause further simplification".

:commit
	a rdf:Property;
	rdfs:domain log:Formula;
	rdfs:range log:Formula;
	rdfs:comment "the LHS builtin constraints are a precondition on the applicability of the rule".

:rewrite
	a rdf:Property;
	rdfs:domain log:Formula;
	rdfs:range log:Formula;
	rdfs:comment "only rewrite RHS user constraints in a simplification rule".
