@prefix log: <http://www.w3.org/2000/10/swap/log#>.
@prefix owl: <http://www.w3.org/2002/07/owl#>.
@prefix rdfs: <http://www.w3.org/2000/01/rdf-schema#>.
@prefix xsd: <http://www.w3.org/2001/XMLSchema#>.
@prefix dce: <http://purl.org/dc/elements/1.1/>.
@prefix skos: <http://www.w3.org/2004/02/skos/core#>.
@prefix event: <http://eulersharp.sourceforge.net/2003/03swap/event#>.
@prefix clinobs: <http://www.agfa.com/w3c/2009/clinicalObservation#>.
@prefix computer: <http://eulersharp.sourceforge.net/2003/03swap/computer#>.
@prefix digproc: <http://eulersharp.sourceforge.net/2003/03swap/digitalProcedure#>.
@prefix quant: <http://eulersharp.sourceforge.net/2003/03swap/quantities#>.
@prefix decisionsupport: <http://eulersharp.sourceforge.net/2003/03swap/decisionSupport#>.

<http://eulersharp.sourceforge.net/2003/03swap/decisionSupport>
	a owl:Ontology;
	dce:title """Decision Support"""@en;
	dce:creator """Hans Cools, MD; Agfa Healthcare, Belgium"""@en;
	dce:contributor """Kristof Depraetere; Agfa Healthcare, Belgium"""@en;
	dce:publisher """Agfa Healthcare, Belgium"""@en;
	dce:description """Formal description of decision support."""@en;
	dce:format """OWL Full"""@en.

#
# CLASSES
#

decisionsupport:Request	# TBD
	a rdfs:Class;
	rdfs:isDefinedBy <http://eulersharp.sourceforge.net/2003/03swap/decisionSupport#>;
	rdfs:label """decision support request"""@en;
	rdfs:subClassOf digproc:Request.			

decisionsupport:ClinicalRequest # TBD
	a rdfs:Class;
	rdfs:isDefinedBy <http://eulersharp.sourceforge.net/2003/03swap/decisionSupport#>;
	rdfs:label """clinical decision support request"""@en;
	rdfs:subClassOf decisionsupport:Request, [
		a owl:Restriction; owl:onProperty decisionsupport:hasObservablesResultFormula; owl:someValuesFrom decisionsupport:ClinicalObservablesResultFormula].

decisionsupport:ResultFormula
	a rdfs:Class;
	rdfs:isDefinedBy <http://eulersharp.sourceforge.net/2003/03swap/decisionSupport#>;
	rdfs:label """decision support result formula"""@en;
	skos:definition """Formula related to its literal form expressing patient state in triples, as input for clinical decision support."""@en;	
	rdfs:subClassOf log:Formula.

decisionsupport:ObservablesResultFormula
	a rdfs:Class;
	rdfs:isDefinedBy <http://eulersharp.sourceforge.net/2003/03swap/decisionSupport#>;
	rdfs:label """decision support observables result formula"""@en;
	skos:definition """Formula related to its literal form expressing findings in boolean (nested) triples, as input for decision support."""@en;
	rdfs:subClassOf log:Formula, [
		a owl:Restriction; owl:onProperty log:n3String; owl:someValuesFrom log:String], [
		a owl:Restriction; owl:onProperty event:hasObject; owl:someValuesFrom event:Finding].

decisionsupport:ClinicalObservablesResultFormula
	a rdfs:Class;
	rdfs:isDefinedBy <http://eulersharp.sourceforge.net/2003/03swap/decisionSupport#>;
	rdfs:label """clinical decision support observables result formula"""@en;
	skos:definition """Formula related to its literal form expressing clinical findings in boolean (nested) triples, as input for clinical decision support."""@en;
	rdfs:subClassOf decisionsupport:ObservablesResultFormula, [
		a owl:Restriction; owl:onProperty log:n3String; owl:someValuesFrom log:String], [
		a owl:Restriction; owl:onProperty event:hasObject; owl:someValuesFrom clinobs:Finding].

decisionsupport:StateResultFormula
	a rdfs:Class;
	rdfs:isDefinedBy <http://eulersharp.sourceforge.net/2003/03swap/decisionSupport#>;
	rdfs:label """decision support state result formula"""@en;
	skos:definition """Formula related to its literal form expressing state of something in triples, as object of a clinical decision support request."""@en;
	rdfs:subClassOf log:Formula.

decisionsupport:PatientStateResultFormula
	a rdfs:Class;
	rdfs:isDefinedBy <http://eulersharp.sourceforge.net/2003/03swap/decisionSupport#>;
	rdfs:label """decision support patient state result formula"""@en;
	skos:definition """Formula related to its literal form expressing patient state in triples, as input for clinical decision support."""@en;
	rdfs:subClassOf decisionsupport:StateResultFormula.

decisionsupport:Belief
	a rdfs:Class;
	rdfs:isDefinedBy <http://eulersharp.sourceforge.net/2003/03swap/decisionSupport#>;
	rdfs:label """belief probability"""@en;
	skos:definition """Calculated probability of a belief in something."""@en;
	rdfs:subClassOf quant:Probability, [
		a owl:Restriction; owl:onProperty quant:hasMeasurement; owl:someValuesFrom [
			a owl:Restriction; owl:onProperty quant:hasValue; owl:someValuesFrom xsd:double]].

# TherapyTheory, DiagnosisTheory

# evidence, hypothesis
# MD: date, author, quality rank

#
# PROPERTIES
#

# decisionsupport:hasStrategy
#	a owl:ObjectProperty;
#	rdfs:isDefinedBy <http://eulersharp.sourceforge.net/2003/03swap/decisionSupport#>;
#	skos:definition """Specifying a strategy for a decision support request."""@en;
#	rdfs:domain decisionsupport:Request;
#	rdfs:range decisionsupport:Strategy.

decisionsupport:hasObservablesResultFormula
	a owl:ObjectProperty;
	rdfs:isDefinedBy <http://eulersharp.sourceforge.net/2003/03swap/decisionSupport#>;
	skos:definition """Specifying an observables result formula for a decision support request."""@en;
	rdfs:domain decisionsupport:Request;
	rdfs:range decisionsupport:ObservablesResultFormula.

decisionsupport:hasPatientStateResultFormula
	a owl:ObjectProperty;
	rdfs:isDefinedBy <http://eulersharp.sourceforge.net/2003/03swap/decisionSupport#>;
	skos:definition """Specifying a patient state result formula for a clinical decision support request."""@en;
	rdfs:domain decisionsupport:ClinicalRequest;
	rdfs:range decisionsupport:PatientStateResultFormula.

decisionsupport:hasResultFormula
	a owl:ObjectProperty;
	rdfs:isDefinedBy <http://eulersharp.sourceforge.net/2003/03swap/decisionSupport#>;
	skos:definition """Specifying a result formula for a decision support request."""@en;
	rdfs:domain decisionsupport:Request;
	rdfs:range decisionsupport:ResultFormula.

decisionsupport:beliefIn
	a owl:ObjectProperty;
	rdfs:isDefinedBy <http://eulersharp.sourceforge.net/2003/03swap/decisionSupport#>;
	skos:definition """Specifying something that has a belief probability, e.g. a clinical therapy that is believed to be performed with a certain chance of being successful."""@en;
	rdfs:domain decisionsupport:Belief;
	skos:note """rdfs:range not specified, because it can be virtually anything; e.g. http://www.agfa.com/w3c/2009/therapy#Therapy (clinical therapy)."""@en;
	rdfs:comment """E.g. ([quant:hasValue 9.660533530762310e-001]) decisionsupport:beliefIn i:Lomefloxacin_400mg_PO_UID_3D."""@en.

decisionsupport:hasBelief
	a owl:ObjectProperty;
	rdfs:isDefinedBy <http://eulersharp.sourceforge.net/2003/03swap/decisionSupport#>;
	skos:definition """Specifying a belief probability of something, e.g. a clinical therapy."""@en;
	rdfs:range decisionsupport:Belief;
	skos:note """rdfs:domain not specified, because it can be virtually anything; e.g. http://www.agfa.com/w3c/2009/therapy#Therapy (clinical therapy)."""@en;
	owl:inverseOf decisionsupport:beliefIn.
